Use functions from variables for interpretation of contexts in Fμref

F_mu_ref/typing.v
@@ -1,3 +1,4 @@
+Require Import prelude.base.
 Require Import F_mu_ref.lang.
 
 Inductive type :=
@@ -16,329 +17,44 @@ Instance Rename_type : Rename type. derive. Defined.
 Instance Subst_type : Subst type. derive. Defined.
 Instance SubstLemmas_typer : SubstLemmas type. derive. Qed.
 
-Inductive closed_type (k : nat) : type → Prop :=
-| CLT_TUnit : closed_type k TUnit
-| CLT_TProd t t' : closed_type k t → closed_type k t' → closed_type k (TProd t t')
-| CLT_TSum t t' : closed_type k t → closed_type k t' → closed_type k (TSum t t')
-| CLT_TArrow t t' : closed_type k t → closed_type k t' → closed_type k (TArrow t t')
-| CLT_TRec t : closed_type (S k) t → closed_type k (TRec t)
-| CLT_TVar n : n < k → closed_type k (TVar n)
-| CLT_TForall t : closed_type (S k) t → closed_type k (TForall t)
-| CLT_Tref t : closed_type k t → closed_type k (Tref t)
-.
-
-Hint Constructors closed_type.
-
-Lemma closed_type_prod_1 {k : nat} {τ1 τ2 : type} :
-  closed_type k (TProd τ1 τ2) → closed_type k τ1.
-Proof. intros H; inversion H; subst; trivial. Qed.
-
-Lemma closed_type_prod_2 {k : nat} {τ1 τ2 : type} :
-  closed_type k (TProd τ1 τ2) → closed_type k τ2.
-Proof. intros H; inversion H; subst; trivial. Qed.
-
-Lemma closed_type_sum_1 {k : nat} {τ1 τ2 : type} :
-  closed_type k (TSum τ1 τ2) → closed_type k τ1.
-Proof. intros H; inversion H; subst; trivial. Qed.
-
-Lemma closed_type_sum_2 {k : nat} {τ1 τ2 : type} :
-  closed_type k (TSum τ1 τ2) → closed_type k τ2.
-Proof. intros H; inversion H; subst; trivial. Qed.
-
-Lemma closed_type_arrow_1 {k : nat} {τ1 τ2 : type} :
-  closed_type k (TArrow τ1 τ2) → closed_type k τ1.
-Proof. intros H; inversion H; subst; trivial. Qed.
-
-Lemma closed_type_arrow_2 {k : nat} {τ1 τ2 : type} :
-  closed_type k (TArrow τ1 τ2) → closed_type k τ2.
-Proof. intros H; inversion H; subst; trivial. Qed.
-
-Lemma closed_type_rec {k : nat} {τ : type} :
-  closed_type k (TRec τ) → closed_type (S k) τ.
-Proof. intros H; inversion H; subst; trivial. Qed.
-
-Lemma closed_type_var {k : nat} {v : var} :
-  closed_type k (TVar v) → v < k.
-Proof. intros H; inversion H; subst; trivial. Qed.
-
-Lemma closed_type_forall {k : nat} {τ : type} :
-  closed_type k (TForall τ) → closed_type (S k) τ.
-Proof. intros H; inversion H; subst; trivial. Qed.
-
-Lemma closed_type_ref {k : nat} {τ : type} :
-  closed_type k (Tref τ) → closed_type k τ.
-Proof. intros H; inversion H; subst; trivial. Qed.
-
-Local Hint Resolve closed_type_prod_1 closed_type_prod_2 closed_type_sum_1
-      closed_type_sum_2 closed_type_arrow_1 closed_type_arrow_2
-      closed_type_rec closed_type_var closed_type_forall closed_type_ref.
-
-Lemma closed_type_S (k : nat) (τ : type) : closed_type k τ → closed_type (S k) τ.
-Proof. intros H; induction H; auto using closed_type with omega. Qed.
-
-Lemma closed_type_le (k k' : nat) (τ : type) : k ≤ k' → closed_type k τ → closed_type k' τ.
-Proof. intros H; induction H; auto using closed_type, closed_type_S with omega. Qed.
-
-Definition closed_ctx (k : nat) (Γ : list type) := Forall (closed_type k) Γ.
-
-Lemma closed_ctx_S (k : nat) (Γ : list type) : closed_ctx k Γ → closed_ctx (S k) Γ.
-Proof. intros H. eapply Forall_impl; [| apply closed_type_S]; trivial. Qed.
-
-Lemma closed_ctx_le (k k' : nat) (Γ : list type) : k ≤ k' → closed_ctx k Γ → closed_ctx k' Γ.
-Proof. intros H; induction H; auto using closed_type, closed_ctx_S with omega. Qed.
-
-Lemma closed_ctx_closed_type (k : nat) (Γ : list type) (x : var) (τ : type) :
-  closed_ctx k Γ → Γ !! x = Some τ → closed_type k τ.
-Proof. intros; eapply Forall_lookup; eauto. Qed.
-
-Lemma closed_ctx_map (k k' : nat) (Γ : list type) (f : type → type) :
-  closed_ctx k Γ →
-  (∀ τ, closed_type k τ → closed_type k' (f τ)) →
-  closed_ctx k' (map f Γ).
-Proof.
-  revert k k' f.
-  induction Γ; intros k k' f H1 H2; cbn; constructor;
-  inversion H1; subst; auto.
-  eapply IHΓ; eauto.
-Qed.
-
-Program Fixpoint zipwith_Forall {A : Type} {P : A → Prop} (l : list A) (H : Forall P l) :
-  list ({x : A | P x}) :=
-  match l as u return Forall P u → _ with
-  | [] => λ _, []
-  | a :: l' => λ H, (a ↾ _) :: (zipwith_Forall l' _)
-  end H.
-Solve Obligations with repeat intros ?; match goal with [H : Forall _ _ |- _] => inversion H; trivial end.
-
-Lemma zipwith_Forall_lookup {A : Type} {P : A → Prop} (l : list A) (Hf : Forall P l) (x : A) (n : nat) :
-  l !! n = Some x → {Hx : P x| (zipwith_Forall l Hf) !! n = Some (x ↾ Hx)}.
-Proof.
-  revert n.
-  induction l; intros n H1; cbn in *; [inversion H1|].
-  destruct n; [cbn in *; inversion H1; subst|]; eauto.
-Qed.
-  
-Definition closed_ctx_list (k : nat) (Γ : list type) (H : closed_ctx k Γ) :
-  list ({τ : type | closed_type k τ}) := zipwith_Forall Γ H.
-
-Inductive typed (k : nat) (Γ : list type) : expr → type → Prop :=
-| Var_typed x τ : (closed_ctx k Γ) → Γ !! x = Some τ → typed k Γ (Var x) τ
-| Unit_typed : closed_ctx k Γ → typed k Γ Unit TUnit
+Inductive typed (Γ : list type) : expr → type → Prop :=
+| Var_typed x τ : Γ !! x = Some τ → typed Γ (Var x) τ
+| Unit_typed : typed Γ Unit TUnit
 | Pair_typed e1 e2 τ1 τ2 :
-    typed k Γ e1 τ1 → typed k Γ e2 τ2 → typed k Γ (Pair e1 e2) (TProd τ1 τ2)
-| Fst_typed e τ1 τ2 : typed k Γ e (TProd τ1 τ2) → typed k Γ (Fst e) τ1
-| Snd_typed e τ1 τ2 : typed k Γ e (TProd τ1 τ2) → typed k Γ (Snd e) τ2
-| InjL_typed e τ1 τ2 : typed k Γ e τ1 → closed_type k τ2 → typed k Γ (InjL e) (TSum τ1 τ2)
-| InjR_typed e τ1 τ2 : typed k Γ e τ2 → closed_type k τ1 → typed k Γ (InjR e) (TSum τ1 τ2)
+    typed Γ e1 τ1 → typed Γ e2 τ2 → typed Γ (Pair e1 e2) (TProd τ1 τ2)
+| Fst_typed e τ1 τ2 : typed Γ e (TProd τ1 τ2) → typed Γ (Fst e) τ1
+| Snd_typed e τ1 τ2 : typed Γ e (TProd τ1 τ2) → typed Γ (Snd e) τ2
+| InjL_typed e τ1 τ2 : typed Γ e τ1 → typed Γ (InjL e) (TSum τ1 τ2)
+| InjR_typed e τ1 τ2 : typed Γ e τ2 → typed Γ (InjR e) (TSum τ1 τ2)
 | Case_typed e0 e1 e2 τ1 τ2 ρ :
-    typed k Γ e0 (TSum τ1 τ2) →
-    typed k (τ1 :: Γ) e1 ρ → typed k (τ2 :: Γ) e2 ρ →
-    typed k Γ (Case e0 e1 e2) ρ
+    typed Γ e0 (TSum τ1 τ2) →
+    typed (τ1 :: Γ) e1 ρ → typed (τ2 :: Γ) e2 ρ →
+    typed Γ (Case e0 e1 e2) ρ
 | Lam_typed e τ1 τ2 :
-    typed k (τ1 :: Γ) e τ2 → typed k Γ (Lam e) (TArrow τ1 τ2)
+    typed (τ1 :: Γ) e τ2 → typed Γ (Lam e) (TArrow τ1 τ2)
 | App_typed e1 e2 τ1 τ2 :
-    typed k Γ e1 (TArrow τ1 τ2) → typed k Γ e2 τ1 → typed k Γ (App e1 e2) τ2
+    typed Γ e1 (TArrow τ1 τ2) → typed Γ e2 τ1 → typed Γ (App e1 e2) τ2
 | TLam_typed e τ :
-    typed (S k) (map (λ t, t.[ren (+1)]) Γ) e τ →
-    typed k Γ (TLam e) (TForall τ)
+    typed (map (λ t, t.[ren (+1)]) Γ) e τ →
+    typed Γ (TLam e) (TForall τ)
 | TApp_typed e τ τ':
-    typed k Γ e (TForall τ) → closed_type k τ' → typed k Γ (TApp e) (τ.[τ'/])
+    typed Γ e (TForall τ) → typed Γ (TApp e) (τ.[τ'/])
 | TFold e τ :
-    typed (S k) (map (λ t, t.[ren (+1)]) Γ) e τ →
-    typed k Γ (Fold e) (TRec τ)
-| TUnfold e τ : typed k Γ e (TRec τ) → typed k Γ (Unfold e) (τ.[(TRec τ)/])
-| TAlloc e τ : typed k Γ e τ → typed k Γ (Alloc e) (Tref τ)
-| TLoad e τ : typed k Γ e (Tref τ) → typed k Γ (Load e) τ
+    typed (map (λ t, t.[ren (+1)]) Γ) e τ →
+    typed Γ (Fold e) (TRec τ)
+| TUnfold e τ : typed Γ e (TRec τ) → typed Γ (Unfold e) (τ.[(TRec τ)/])
+| TAlloc e τ : typed Γ e τ → typed Γ (Alloc e) (Tref τ)
+| TLoad e τ : typed Γ e (Tref τ) → typed Γ (Load e) τ
 | TStore e e' τ :
-    typed k Γ e (Tref τ) → typed k Γ e' τ → typed k Γ (Store e e') TUnit
+    typed Γ e (Tref τ) → typed Γ e' τ → typed Γ (Store e e') TUnit
 .
-
-Lemma closed_type_subst_invariant k τ s1 s2 :
-  closed_type k τ → (∀ x, x < k → s1 x = s2 x) → τ.[s1] = τ.[s2].
-Proof.
-  intros Htyped; revert s1 s2.
-  assert (∀ {A} `{Ids A} `{Rename A}
-            (s1 s2 : nat → A) x, (x ≠ 0 → s1 (pred x) = s2 (pred x)) → up s1 x = up s2 x).
-  { intros A H1 H2. rewrite /up=> s1 s2 [|x] //=; auto with f_equal omega. }
-  induction Htyped => s1 s2 Hs; f_equal/=; eauto using lookup_lt_Some with omega.
-Qed.
-
-Fixpoint iter (n : nat) `(f : A → A) :=
-  match n with
-  | O => λ x, x
-  | S n' => λ x, f (iter n' f x)
-  end.
-
-Lemma iter_S (n : nat) `(f : A → A) (x : A) : iter (S n) f x = iter n f (f x).
-Proof.
-  induction n; cbn; trivial.
-  rewrite -IHn; trivial.
-Qed.
-  
-Lemma iter_upren (m x : nat) f : iter m upren f x = if lt_dec x m then x else m + (f (x - m)).
-Proof.
-  revert x; induction m; cbn; auto with omega.
-  intros x; destruct x; cbn; trivial.
-  rewrite IHm; repeat destruct lt_dec; auto with omega.  
-Qed.
-  
-Lemma iter_up (m x : nat) (f : var → type) : iter m up f x = if lt_dec x m then ids x else rename (+m) (f (x - m)).
-Proof.
-  revert x; induction m; cbn; auto with omega.
-  intros x; destruct x; cbn; asimpl; trivial.
-  intros x; destruct x; cbn; asimpl; trivial.
-  rewrite IHm; repeat destruct lt_dec; auto with omega.
-  asimpl; trivial.
-Qed.
-
-Lemma closed_type_S_ren1:
-  ∀ (τ : type) (n m : nat) (k : nat) (Hle : m ≤ k),
-    (closed_type (n + k) τ.[ren ((iter m upren) (+n))] → closed_type k τ).
-Proof.
-  induction τ; intros n m k Hle H; inversion H; subst; constructor; eauto 2 with omega;
-  try eapply (IHτ n (S m)); asimpl in *; auto with omega.
-  rewrite iter_upren in H1; destruct lt_dec; cbn in *; omega.
-Qed.
-
-Lemma closed_type_S_ren2:
-  ∀ (τ : type) (n m : nat) (k : nat),
-    (closed_type k τ → closed_type (n + k) τ.[ren ((iter m upren) (+n))]).
-Proof.
-  induction τ; intros n m k H; inversion H; subst; constructor; eauto 2 with omega;
-  try (replace (up (ren (iter m upren (+n)))) with
-    (ren (iter (S m) upren (+n))) by (asimpl; trivial);
-    replace (S (n + k)) with (n + (S k)) by omega; auto with omega).
-  rewrite iter_upren; destruct lt_dec; cbn in *; omega.
-Qed.
-
-Lemma closed_type_pred_ren1:
-  ∀ (τ : type) (n m : nat) (k : nat),
-    (closed_type k τ.[ren ((iter m upren) (λ x, x - n))] → closed_type (n + k) τ).
-Proof.
-  induction τ; intros n m k H; inversion H; subst; constructor; eauto 2 with omega;  
-  try (replace (S (n + k)) with (n + (S k)) by omega;
-  apply IHτ with (S m);
-  replace (up (ren (iter m upren (λ x, x - n)))) with
-  (ren (iter (S m) upren (λ x, x - n))) in H1 by (asimpl; trivial); trivial).
-  rewrite iter_upren in H1; destruct lt_dec; omega.
-Qed.
-
-Lemma closed_type_pred_ren2:
-  ∀ (τ : type) (n m : nat) (k : nat) (Hle : m < k),
-    closed_type (n + k) τ → closed_type k τ.[ren ((iter m upren) (λ x, x - n))].
-Proof.
-  induction τ; intros n m k Hle H; inversion H; subst; constructor; eauto 2 with omega;
-  try (replace (up (ren (iter m upren (λ x, x - n)))) with
-    (ren (iter (S m) upren (λ x, x - n))) by (asimpl; trivial); trivial;
-    eapply (IHτ n (S m)); asimpl in *; auto with omega).
-  rewrite iter_upren; destruct lt_dec; omega.
-Qed.
-
-Lemma closed_ctx_map_S:
-  ∀ (k : nat) (Γ : list type), closed_ctx (S k) (map (λ t : type, t.[ren (+1)]) Γ) → closed_ctx k Γ.
-Proof.
-  intros k Γ H.
-  induction Γ; constructor; inversion H; subst.
-  eapply closed_type_S_ren1 with 1 0; cbn; auto with omega.
-  apply IHΓ; trivial.
-Qed.
-
-Lemma closed_type_subst_up_subst (m : nat) (k : nat) (τ : {bind type}) (τ' : type) :
-  closed_type k τ' → closed_type (m + k) τ → closed_type (m + k) τ.[iter m up (τ' .: ids)].
-Proof.
-  revert m k τ'.
-  induction τ; intros m k τ' H1 H2; try constructor; inversion H2; subst; auto;
-  try (change (up (iter m up (τ' .: ids))) with (iter (S m) up (τ' .: ids));
-        change (S (m + k)) with (S m + k);
-        apply IHτ; cbn; auto using closed_type_S).
-  cbn; rewrite iter_up; destruct lt_dec.
-  constructor; auto.
-  asimpl; apply (closed_type_S_ren2 _ m 0).
-  remember (x - m) as u; destruct u; try constructor; auto with omega.
-Qed.
-
-Lemma closed_type_all_closed_subst (m k : nat) (τ : type) (f : var → type) :
-  (∀ x, closed_type k (f x)) → closed_type (m + k) τ.[iter m up f].
-Proof.
-  revert m k.
-  induction τ; intros m k H; try constructor; auto;
-  try (change (up (iter m up f)) with (iter (S m) up f);
-        change (S (m + k)) with (S m + k);
-        apply IHτ; cbn; auto using closed_type_S).
-  cbn; rewrite iter_up; destruct lt_dec.
-  constructor; auto with omega.
-  asimpl; apply (closed_type_S_ren2 _ m 0); trivial.
-Qed.
-
-Lemma closed_type_rel_closed_subst (n k : nat) (τ : type) (f : var → type) :
-  (∀ x, x < n → closed_type k (f x)) → closed_type n τ → closed_type k τ.[f].
-Proof.
-  revert f n k.
-  induction τ; intros f n k H1 H2; inversion H2; subst; try constructor; cbn; auto;
-  try ((eapply IHτ + eapply IHτ1 + eapply IHτ2); cbn; eauto 2 using closed_type_S; fail);
-  try (eapply IHτ; eauto 2;
-       intros x Hx; destruct x; asimpl;
-       try constructor; auto using (closed_type_S_ren2 _ 1 0) with omega).
-Qed.
-
-Lemma closed_type_subst_wiht_up (k m : nat) (τ : type) (τ' : type) :
-  m ≤ k → closed_type (k - m) τ' → closed_type (S k) τ →
-  closed_type k τ.[iter m up (τ' .: ids)].
-Proof.
-  revert k m τ'.
-  induction τ; intros k m τ' Hlt H1 H2; inversion H2; subst; try constructor; auto.
-  - change (up (iter m up (τ' .: ids))) with (iter (S m) up (τ' .: ids));
-    apply IHτ; auto with omega.
-  - cbn.
-    rewrite iter_up.
-    destruct lt_dec.
-    + auto with omega.
-    + asimpl.
-      remember (x - m) as u.
-      destruct u; cbn in *.
-      * replace k with (m + (k - m)) by omega.
-        apply (closed_type_S_ren2 _ m 0); trivial.
-      * asimpl; constructor; omega.
-  - change (up (iter m up (τ' .: ids))) with (iter (S m) up (τ' .: ids));
-    apply IHτ; auto with omega.
-Qed.
-
-Lemma closed_type_subst (k : nat) (τ : type) (τ' : type) :
-  closed_type k τ' → closed_type (S k) τ → closed_type k τ.[τ'/].
-Proof.
-  intros H1 H2.
-  apply (closed_type_subst_wiht_up _ 0);
-    try replace (k - 0) with k; auto with omega.
-Qed.
-
-Lemma typed_closed_ctx_closed_type (k : nat) (Γ : list type) (e : expr) (τ : type) :
-  typed k Γ e τ → closed_ctx k Γ ∧ closed_type k τ.
-Proof.
-  intros H; induction H; intuition; eauto 3 using closed_ctx_closed_type;
-  match goal with
-  | [H : closed_ctx _ (_ :: _) |- _] =>
-    inversion H; clear H; subst;
-    auto
-  | [H : closed_type _ _ |- _] =>
-    inversion H; clear H; subst;
-    auto using closed_ctx_map_S, closed_type_subst
-  end.
-Qed.
-
-Lemma typed_closed_ctx (k : nat) (Γ : list type) (e : expr) (τ : type) :
-  typed k Γ e τ → closed_ctx k Γ.
-Proof. apply typed_closed_ctx_closed_type. Qed.
-
-Lemma typed_closed_type (k : nat) (Γ : list type) (e : expr) (τ : type) :
-  typed k Γ e τ → closed_type k τ.
-Proof. apply typed_closed_ctx_closed_type. Qed.
 
 Local Hint Extern 1 =>
 match goal with [H : context [length (map _ _)] |- _] => rewrite map_length in H end
 : typed_subst_invariant.
 
-Lemma typed_subst_invariant k Γ e τ s1 s2 :
-  typed k Γ e τ → (∀ x, x < length Γ → s1 x = s2 x) → e.[s1] = e.[s2].
+Lemma typed_subst_invariant Γ e τ s1 s2 :
+  typed Γ e τ → (∀ x, x < length Γ → s1 x = s2 x) → e.[s1] = e.[s2].
 Proof.
   intros Htyped; revert s1 s2.
   assert (∀ {A} `{Ids A} `{Rename A}
@@ -347,12 +63,38 @@ Proof.
   induction Htyped => s1 s2 Hs; f_equal/=; eauto using lookup_lt_Some with omega typed_subst_invariant.
 Qed.
 
-Lemma closed_ctx_map_S_back (k : nat) (Γ : list type) (e : expr) (τ : type) :
-  closed_ctx k Γ →
-  closed_ctx (S k) (map (λ t : type, t.[ren (+1)]) Γ).
+Definition env_subst (vs : list val) (x : var) : expr :=
+  from_option (Var x) (of_val <$> vs !! x).
+
+Notation "# v" := (of_val v) (at level 20).
+
+Lemma typed_subst_head_simpl Δ τ e w ws :
+  typed Δ e τ -> List.length Δ = S (List.length ws) →
+  e.[# w .: env_subst ws] = e.[env_subst (w :: ws)]
+.
 Proof.
-  intros H.
-  eapply closed_ctx_map; [eassumption|].
-  clear; intros τ' H'.
-  set (HW := closed_type_S_ren2 τ' 1 0); cbn in HW; apply HW; trivial.
+  intros H1 H2.
+  rewrite /env_subst. eapply typed_subst_invariant; eauto=> /= -[|x] ? //=.
+  destruct (lookup_lt_is_Some_2 ws x) as [v' Hv]; first omega; simpl.
+    by rewrite Hv.
+Qed.
+
+
+Local Opaque eq_nat_dec.
+
+Lemma iter_up_subst_type (m : nat) (τ : type) (x : var) :
+  (iter m up (τ .: ids) x) =
+  if lt_dec x m then ids x else
+    if eq_nat_dec x m then τ.[ren (+m)] else ids (x - 1).
+Proof.
+  revert x τ.
+  induction m; intros x τ; cbn.
+  - destruct x; cbn.
+    + destruct eq_nat_dec; auto with omega.
+      asimpl; trivial.
+    + destruct eq_nat_dec; auto with omega.
+  - destruct x; asimpl; trivial.
+    rewrite IHm.
+    repeat destruct lt_dec; repeat destruct eq_nat_dec;
+      asimpl; auto with omega.
 Qed.
